securedrop-protocol/protocol-minimal/src/primitives/provider.rs
@@ -58,7 +58,9 @@ pub mod ed25519 {
 
     /// Derive the Ed25519 public key from a secret key.
     #[cfg_attr(hax, hax_lib::opaque)]
-    pub(crate) use libcrux_ed25519::secret_to_public;
+    pub(crate) fn secret_to_public(public_key: &mut [u8; 32], secret_key: &[u8; 32]) {
+        libcrux_ed25519::secret_to_public(public_key, secret_key)
+    }
 }
 
 pub mod rng {
