securedrop-protocol/protocol-minimal/proofs/fstar/extraction/Securedrop_protocol_minimal.Journalist.fst
@@ -6,10 +6,12 @@ open Core_models
 let _ =
   (* This module has implicit dependencies, here we make them explicit. *)
   (* The implicit dependencies arise from typeclasses instances. *)
+  let open Anyhow.Error in
   let open Rand_core in
   let open Securedrop_protocol_minimal.Keys in
   let open Securedrop_protocol_minimal.Message in
   let open Securedrop_protocol_minimal.Primitives.X25519 in
+  let open Securedrop_protocol_minimal.Sign in
   let open Securedrop_protocol_minimal.Traits in
   ()
 
@@ -463,6 +465,74 @@ let impl_5: Securedrop_protocol_minimal.Traits.t_Enrollable t_Journalist =
     fun (self: t_Journalist) -> self.f_signing_key.Securedrop_protocol_minimal.Keys.f_pk
   }
 
+#push-options "--admit_smt_queries true"
+
+/// Generate one ephemeral key bundle and sign its pubkeys.
+let make_signed_bundle
+      (#v_R: Type0)
+      (#[FStar.Tactics.Typeclasses.tcresolve ()] i0: Rand_core.t_RngCore v_R)
+      (#[FStar.Tactics.Typeclasses.tcresolve ()] i1: Rand_core.t_CryptoRng v_R)
+      (rng: v_R)
+      (signing_key: Securedrop_protocol_minimal.Sign.t_SigningKey)
+    : (v_R & Securedrop_protocol_minimal.Keys.t_SignedMessageKeyBundle) =
+  let
+  (tmp0: v_R),
+  (out:
+    Core_models.Result.t_Result Securedrop_protocol_minimal.Message.t_MessageKeyPair Anyhow.t_Error)
+  =
+    Securedrop_protocol_minimal.Message.keygen #v_R rng
+  in
+  let rng:v_R = tmp0 in
+  let apke_kp:Securedrop_protocol_minimal.Message.t_MessageKeyPair =
+    Core_models.Result.impl__expect #Securedrop_protocol_minimal.Message.t_MessageKeyPair
+      #Anyhow.t_Error
+      out
+      "SD-APKE ephemeral keygen failed"
+  in
+  let
+  (tmp0: v_R),
+  (out:
+    Core_models.Result.t_Result Securedrop_protocol_minimal.Metadata.t_MetadataKeyPair
+      Anyhow.t_Error) =
+    Securedrop_protocol_minimal.Metadata.keygen #v_R rng
+  in
+  let rng:v_R = tmp0 in
+  let metadata_kp:Securedrop_protocol_minimal.Metadata.t_MetadataKeyPair =
+    Core_models.Result.impl__expect #Securedrop_protocol_minimal.Metadata.t_MetadataKeyPair
+      #Anyhow.t_Error
+      out
+      "Failed to generate metadata keys"
+  in
+  let bundle:Securedrop_protocol_minimal.Keys.t_MessageKeyBundle =
+    Securedrop_protocol_minimal.Keys.impl_MessageKeyBundle__new apke_kp metadata_kp
+  in
+  let pubkey_bytes:Alloc.Vec.t_Vec u8 Alloc.Alloc.t_Global =
+    Securedrop_protocol_minimal.Keys.impl_KeyBundlePublic__as_bytes (Securedrop_protocol_minimal.Keys.impl_MessageKeyBundle__public
+          bundle
+        <:
+        Securedrop_protocol_minimal.Keys.t_KeyBundlePublic)
+  in
+  let
+  (selfsig:
+    Securedrop_protocol_minimal.Sign.t_Signature
+    Securedrop_protocol_minimal.Sign.t_JournalistEphemeralKey):Securedrop_protocol_minimal.Sign.t_Signature
+  Securedrop_protocol_minimal.Sign.t_JournalistEphemeralKey =
+    Securedrop_protocol_minimal.Sign.impl_SigningKey__sign #Securedrop_protocol_minimal.Sign.t_JournalistEphemeralKey
+      signing_key
+      (Alloc.Vec.impl_1__as_slice pubkey_bytes <: t_Slice u8)
+  in
+  let hax_temp_output:Securedrop_protocol_minimal.Keys.t_SignedMessageKeyBundle =
+    {
+      Securedrop_protocol_minimal.Keys.f_bundle = bundle;
+      Securedrop_protocol_minimal.Keys.f_selfsig = selfsig
+    }
+    <:
+    Securedrop_protocol_minimal.Keys.t_SignedMessageKeyBundle
+  in
+  rng, hax_temp_output <: (v_R & Securedrop_protocol_minimal.Keys.t_SignedMessageKeyBundle)
+
+#pop-options
+
 assume
 val impl_Journalist__new':
     #v_R: Type0 ->
@@ -484,3 +554,497 @@ val impl_Journalist__public': self: t_Journalist -> idx: usize -> t_JournalistPu
 
 unfold
 let impl_Journalist__public = impl_Journalist__public'
+
+/// Generate `n` fresh signed ephemeral key bundles and retain them in memory.
+/// The public halves are uploaded to the server via
+/// [`create_ephemeral_key_request`](crate::api::JournalistApi::create_ephemeral_key_request).
+/// The secret halves should be persisted via [`Journalist::ephemeral_bundle_bytes`].
+assume
+val impl_Journalist__generate_ephemeral_bundles':
+    #v_R: Type0 ->
+    {| i0: Rand_core.t_RngCore v_R |} ->
+    {| i1: Rand_core.t_CryptoRng v_R |} ->
+    self: t_Journalist ->
+    rng: v_R ->
+    n: usize
+  -> (t_Journalist & v_R)
+
+unfold
+let impl_Journalist__generate_ephemeral_bundles
+      (#v_R: Type0)
+      (#[FStar.Tactics.Typeclasses.tcresolve ()] i0: Rand_core.t_RngCore v_R)
+      (#[FStar.Tactics.Typeclasses.tcresolve ()] i1: Rand_core.t_CryptoRng v_R)
+     = impl_Journalist__generate_ephemeral_bundles' #v_R #i0 #i1
+
+/// Byte representation of a [`Journalist`]'s long-term keypairs, sufficient
+/// to reconstruct the long-term state via
+/// [`Journalist::from_long_term_bytes`].
+type t_JournalistLongTermBytes = {
+  f_sig_seed:t_Array u8 (mk_usize 32);
+  f_fetch_sk:t_Array u8 (mk_usize 32);
+  f_apke_dhakem_sk:t_Array u8 (mk_usize 32);
+  f_apke_mlkem_sk:t_Array u8 (mk_usize 2400);
+  f_apke_mlkem_pk:t_Array u8 (mk_usize 1184)
+}
+
+/// Extract the long-term keypairs as raw bytes, sufficient to
+/// reconstruct the long-term Journalist state via
+/// [`Journalist::from_long_term_bytes`].
+let impl_Journalist__long_term_bytes (self: t_Journalist) : t_JournalistLongTermBytes =
+  {
+    f_sig_seed
+    =
+    Securedrop_protocol_minimal.Sign.impl_SigningKey__as_bytes self.f_signing_key
+        .Securedrop_protocol_minimal.Keys.f_sk;
+    f_fetch_sk
+    =
+    Securedrop_protocol_minimal.Primitives.X25519.impl_DHPrivateKey__as_bytes self.f_fetch_key
+        .Securedrop_protocol_minimal.Keys.f_sk;
+    f_apke_dhakem_sk
+    =
+    Securedrop_protocol_minimal.Primitives.Dh_akem.impl_DhAkemPrivateKey__as_bytes (Securedrop_protocol_minimal.Message.impl_MessageKeyPair__private_key
+          self.f_reply_apke
+        <:
+        Securedrop_protocol_minimal.Message.t_MessagePrivateKey)
+        .Securedrop_protocol_minimal.Message.f_dhakem;
+    f_apke_mlkem_sk
+    =
+    Securedrop_protocol_minimal.Primitives.Mlkem.impl_MLKEM768PrivateKey__as_bytes (Securedrop_protocol_minimal.Message.impl_MessageKeyPair__private_key
+          self.f_reply_apke
+        <:
+        Securedrop_protocol_minimal.Message.t_MessagePrivateKey)
+        .Securedrop_protocol_minimal.Message.f_mlkem;
+    f_apke_mlkem_pk
+    =
+    Securedrop_protocol_minimal.Primitives.Mlkem.impl_MLKEM768PublicKey__as_bytes (Securedrop_protocol_minimal.Message.impl_MessageKeyPair__public_key
+          self.f_reply_apke
+        <:
+        Securedrop_protocol_minimal.Message.t_MessagePublicKey)
+        .Securedrop_protocol_minimal.Message.f_mlkem
+  }
+  <:
+  t_JournalistLongTermBytes
+
+/// Reconstruct the long-term Journalist state from raw key bytes.
+assume
+val impl_Journalist__from_long_term_bytes': parts: t_JournalistLongTermBytes -> t_Journalist
+
+unfold
+let impl_Journalist__from_long_term_bytes = impl_Journalist__from_long_term_bytes'
+
+/// Serialized length of `sig_seed || fetch_sk || apke_dhakem_sk || apke_mlkem_sk || apke_mlkem_pk`.
+let impl_JournalistLongTermBytes__LEN: usize =
+  (((mk_usize 32 +! mk_usize 32 <: usize) +! mk_usize 32 <: usize) +!
+    Securedrop_protocol_minimal.Primitives.Mlkem.v_MLKEM768_PRIVATE_KEY_LEN
+    <:
+    usize) +!
+  Securedrop_protocol_minimal.Primitives.Mlkem.v_MLKEM768_PUBLIC_KEY_LEN
+
+/// Serialize as `sig_seed || fetch_sk || apke_dhakem_sk || apke_mlkem_sk || apke_mlkem_pk`.
+let impl_JournalistLongTermBytes__as_bytes (self: t_JournalistLongTermBytes)
+    : Alloc.Vec.t_Vec u8 Alloc.Alloc.t_Global =
+  let out:Alloc.Vec.t_Vec u8 Alloc.Alloc.t_Global =
+    Alloc.Vec.impl__with_capacity #u8 impl_JournalistLongTermBytes__LEN
+  in
+  let out:Alloc.Vec.t_Vec u8 Alloc.Alloc.t_Global =
+    Alloc.Vec.impl_2__extend_from_slice #u8
+      #Alloc.Alloc.t_Global
+      out
+      (self.f_sig_seed <: t_Slice u8)
+  in
+  let out:Alloc.Vec.t_Vec u8 Alloc.Alloc.t_Global =
+    Alloc.Vec.impl_2__extend_from_slice #u8
+      #Alloc.Alloc.t_Global
+      out
+      (self.f_fetch_sk <: t_Slice u8)
+  in
+  let out:Alloc.Vec.t_Vec u8 Alloc.Alloc.t_Global =
+    Alloc.Vec.impl_2__extend_from_slice #u8
+      #Alloc.Alloc.t_Global
+      out
+      (self.f_apke_dhakem_sk <: t_Slice u8)
+  in
+  let out:Alloc.Vec.t_Vec u8 Alloc.Alloc.t_Global =
+    Alloc.Vec.impl_2__extend_from_slice #u8
+      #Alloc.Alloc.t_Global
+      out
+      (self.f_apke_mlkem_sk <: t_Slice u8)
+  in
+  let out:Alloc.Vec.t_Vec u8 Alloc.Alloc.t_Global =
+    Alloc.Vec.impl_2__extend_from_slice #u8
+      #Alloc.Alloc.t_Global
+      out
+      (self.f_apke_mlkem_pk <: t_Slice u8)
+  in
+  out
+
+/// Deserialize from `sig_seed || fetch_sk || apke_dhakem_sk || apke_mlkem_sk || apke_mlkem_pk` bytes.
+/// # Errors
+/// Returns an error if the byte slice has the incorrect length.
+let impl_JournalistLongTermBytes__from_bytes (bytes: t_Slice u8)
+    : Core_models.Result.t_Result t_JournalistLongTermBytes Anyhow.t_Error =
+  if (Core_models.Slice.impl__len #u8 bytes <: usize) <>. impl_JournalistLongTermBytes__LEN
+  then
+    let args:(usize & usize) =
+      impl_JournalistLongTermBytes__LEN, Core_models.Slice.impl__len #u8 bytes <: (usize & usize)
+    in
+    let args:t_Array Core_models.Fmt.Rt.t_Argument (mk_usize 2) =
+      let list =
+        [
+          Core_models.Fmt.Rt.impl__new_display #usize args._1;
+          Core_models.Fmt.Rt.impl__new_display #usize args._2
+        ]
+      in
+      FStar.Pervasives.assert_norm (Prims.eq2 (List.Tot.length list) 2);
+      Rust_primitives.Hax.array_of_list 2 list
+    in
+    Core_models.Result.Result_Err
+    (Anyhow.Error.impl__msg #Alloc.String.t_String
+        (Core_models.Hint.must_use #Alloc.String.t_String
+            (Alloc.Fmt.format (Core_models.Fmt.Rt.impl_1__new_v1 (mk_usize 2)
+                    (mk_usize 2)
+                    (let list = ["Invalid JournalistLongTermBytes length: expected "; ", got "] in
+                      FStar.Pervasives.assert_norm (Prims.eq2 (List.Tot.length list) 2);
+                      Rust_primitives.Hax.array_of_list 2 list)
+                    args
+                  <:
+                  Core_models.Fmt.t_Arguments)
+              <:
+              Alloc.String.t_String)
+          <:
+          Alloc.String.t_String))
+    <:
+    Core_models.Result.t_Result t_JournalistLongTermBytes Anyhow.t_Error
+  else
+    let (sig_seed: t_Slice u8), (rest: t_Slice u8) =
+      Core_models.Slice.impl__split_at #u8 bytes (mk_usize 32)
+    in
+    let (fetch_sk: t_Slice u8), (rest: t_Slice u8) =
+      Core_models.Slice.impl__split_at #u8 rest (mk_usize 32)
+    in
+    let (apke_dhakem_sk: t_Slice u8), (rest: t_Slice u8) =
+      Core_models.Slice.impl__split_at #u8 rest (mk_usize 32)
+    in
+    let (apke_mlkem_sk: t_Slice u8), (apke_mlkem_pk: t_Slice u8) =
+      Core_models.Slice.impl__split_at #u8
+        rest
+        Securedrop_protocol_minimal.Primitives.Mlkem.v_MLKEM768_PRIVATE_KEY_LEN
+    in
+    Core_models.Result.Result_Ok
+    ({
+        f_sig_seed
+        =
+        Core_models.Result.impl__expect #(t_Array u8 (mk_usize 32))
+          #Core_models.Array.t_TryFromSliceError
+          (Core_models.Convert.f_try_into #(t_Slice u8)
+              #(t_Array u8 (mk_usize 32))
+              #FStar.Tactics.Typeclasses.solve
+              sig_seed
+            <:
+            Core_models.Result.t_Result (t_Array u8 (mk_usize 32))
+              Core_models.Array.t_TryFromSliceError)
+          "wrong checked length";
+        f_fetch_sk
+        =
+        Core_models.Result.impl__expect #(t_Array u8 (mk_usize 32))
+          #Core_models.Array.t_TryFromSliceError
+          (Core_models.Convert.f_try_into #(t_Slice u8)
+              #(t_Array u8 (mk_usize 32))
+              #FStar.Tactics.Typeclasses.solve
+              fetch_sk
+            <:
+            Core_models.Result.t_Result (t_Array u8 (mk_usize 32))
+              Core_models.Array.t_TryFromSliceError)
+          "wrong checked length";
+        f_apke_dhakem_sk
+        =
+        Core_models.Result.impl__expect #(t_Array u8 (mk_usize 32))
+          #Core_models.Array.t_TryFromSliceError
+          (Core_models.Convert.f_try_into #(t_Slice u8)
+              #(t_Array u8 (mk_usize 32))
+              #FStar.Tactics.Typeclasses.solve
+              apke_dhakem_sk
+            <:
+            Core_models.Result.t_Result (t_Array u8 (mk_usize 32))
+              Core_models.Array.t_TryFromSliceError)
+          "wrong checked length";
+        f_apke_mlkem_sk
+        =
+        Core_models.Result.impl__expect #(t_Array u8 (mk_usize 2400))
+          #Core_models.Array.t_TryFromSliceError
+          (Core_models.Convert.f_try_into #(t_Slice u8)
+              #(t_Array u8 (mk_usize 2400))
+              #FStar.Tactics.Typeclasses.solve
+              apke_mlkem_sk
+            <:
+            Core_models.Result.t_Result (t_Array u8 (mk_usize 2400))
+              Core_models.Array.t_TryFromSliceError)
+          "wrong checked length";
+        f_apke_mlkem_pk
+        =
+        Core_models.Result.impl__expect #(t_Array u8 (mk_usize 1184))
+          #Core_models.Array.t_TryFromSliceError
+          (Core_models.Convert.f_try_into #(t_Slice u8)
+              #(t_Array u8 (mk_usize 1184))
+              #FStar.Tactics.Typeclasses.solve
+              apke_mlkem_pk
+            <:
+            Core_models.Result.t_Result (t_Array u8 (mk_usize 1184))
+              Core_models.Array.t_TryFromSliceError)
+          "wrong checked length"
+      }
+      <:
+      t_JournalistLongTermBytes)
+    <:
+    Core_models.Result.t_Result t_JournalistLongTermBytes Anyhow.t_Error
+
+/// Byte representation of one ephemeral key bundle's secret halves
+type t_EphemeralBundleBytes = {
+  f_apke_dhakem_sk:t_Array u8 (mk_usize 32);
+  f_apke_mlkem_sk:t_Array u8 (mk_usize 2400);
+  f_apke_mlkem_pk:t_Array u8 (mk_usize 1184);
+  f_metadata_sk:t_Array u8 (mk_usize 32);
+  f_metadata_pk:t_Array u8 (mk_usize 1216)
+}
+
+/// Extract the secret halves of the retained ephemeral key bundles so we can
+/// reconstruct them via [`Journalist::load_ephemeral_bundles`].
+/// Used by the demo.
+assume
+val impl_Journalist__ephemeral_bundle_bytes': self: t_Journalist
+  -> Alloc.Vec.t_Vec t_EphemeralBundleBytes Alloc.Alloc.t_Global
+
+unfold
+let impl_Journalist__ephemeral_bundle_bytes = impl_Journalist__ephemeral_bundle_bytes'
+
+/// Reconstruct ephemeral key bundles from persisted secret bytes.
+/// Used by the demo
+assume
+val impl_Journalist__load_ephemeral_bundles':
+    self: t_Journalist ->
+    bundles: Alloc.Vec.t_Vec t_EphemeralBundleBytes Alloc.Alloc.t_Global
+  -> t_Journalist
+
+unfold
+let impl_Journalist__load_ephemeral_bundles = impl_Journalist__load_ephemeral_bundles'
+
+/// Serialized length of
+/// `apke_dhakem_sk || apke_mlkem_sk || apke_mlkem_pk || metadata_sk || metadata_pk`.
+let impl_EphemeralBundleBytes__LEN: usize =
+  (((mk_usize 32 +! Securedrop_protocol_minimal.Primitives.Mlkem.v_MLKEM768_PRIVATE_KEY_LEN <: usize
+      ) +!
+      Securedrop_protocol_minimal.Primitives.Mlkem.v_MLKEM768_PUBLIC_KEY_LEN
+      <:
+      usize) +!
+    Securedrop_protocol_minimal.Primitives.Xwing.v_XWING_PRIVATE_KEY_LEN
+    <:
+    usize) +!
+  Securedrop_protocol_minimal.Primitives.Xwing.v_XWING_PUBLIC_KEY_LEN
+
+let impl_EphemeralBundleBytes__from_bundle
+      (bundle: Securedrop_protocol_minimal.Keys.t_MessageKeyBundle)
+    : t_EphemeralBundleBytes =
+  {
+    f_apke_dhakem_sk
+    =
+    Securedrop_protocol_minimal.Primitives.Dh_akem.impl_DhAkemPrivateKey__as_bytes (Securedrop_protocol_minimal.Message.impl_MessageKeyPair__private_key
+          bundle.Securedrop_protocol_minimal.Keys.f_apke
+        <:
+        Securedrop_protocol_minimal.Message.t_MessagePrivateKey)
+        .Securedrop_protocol_minimal.Message.f_dhakem;
+    f_apke_mlkem_sk
+    =
+    Securedrop_protocol_minimal.Primitives.Mlkem.impl_MLKEM768PrivateKey__as_bytes (Securedrop_protocol_minimal.Message.impl_MessageKeyPair__private_key
+          bundle.Securedrop_protocol_minimal.Keys.f_apke
+        <:
+        Securedrop_protocol_minimal.Message.t_MessagePrivateKey)
+        .Securedrop_protocol_minimal.Message.f_mlkem;
+    f_apke_mlkem_pk
+    =
+    Securedrop_protocol_minimal.Primitives.Mlkem.impl_MLKEM768PublicKey__as_bytes (Securedrop_protocol_minimal.Message.impl_MessageKeyPair__public_key
+          bundle.Securedrop_protocol_minimal.Keys.f_apke
+        <:
+        Securedrop_protocol_minimal.Message.t_MessagePublicKey)
+        .Securedrop_protocol_minimal.Message.f_mlkem;
+    f_metadata_sk
+    =
+    Securedrop_protocol_minimal.Metadata.impl_MetadataKeyPair__secret_bytes bundle
+        .Securedrop_protocol_minimal.Keys.f_metadata_kp;
+    f_metadata_pk
+    =
+    Securedrop_protocol_minimal.Metadata.impl_MetadataKeyPair__public_bytes bundle
+        .Securedrop_protocol_minimal.Keys.f_metadata_kp
+  }
+  <:
+  t_EphemeralBundleBytes
+
+assume
+val impl_EphemeralBundleBytes__into_bundle': self: t_EphemeralBundleBytes
+  -> Securedrop_protocol_minimal.Keys.t_MessageKeyBundle
+
+unfold
+let impl_EphemeralBundleBytes__into_bundle = impl_EphemeralBundleBytes__into_bundle'
+
+/// Serialize as
+/// `apke_dhakem_sk || apke_mlkem_sk || apke_mlkem_pk || metadata_sk || metadata_pk`.
+let impl_EphemeralBundleBytes__as_bytes (self: t_EphemeralBundleBytes)
+    : Alloc.Vec.t_Vec u8 Alloc.Alloc.t_Global =
+  let out:Alloc.Vec.t_Vec u8 Alloc.Alloc.t_Global =
+    Alloc.Vec.impl__with_capacity #u8 impl_EphemeralBundleBytes__LEN
+  in
+  let out:Alloc.Vec.t_Vec u8 Alloc.Alloc.t_Global =
+    Alloc.Vec.impl_2__extend_from_slice #u8
+      #Alloc.Alloc.t_Global
+      out
+      (self.f_apke_dhakem_sk <: t_Slice u8)
+  in
+  let out:Alloc.Vec.t_Vec u8 Alloc.Alloc.t_Global =
+    Alloc.Vec.impl_2__extend_from_slice #u8
+      #Alloc.Alloc.t_Global
+      out
+      (self.f_apke_mlkem_sk <: t_Slice u8)
+  in
+  let out:Alloc.Vec.t_Vec u8 Alloc.Alloc.t_Global =
+    Alloc.Vec.impl_2__extend_from_slice #u8
+      #Alloc.Alloc.t_Global
+      out
+      (self.f_apke_mlkem_pk <: t_Slice u8)
+  in
+  let out:Alloc.Vec.t_Vec u8 Alloc.Alloc.t_Global =
+    Alloc.Vec.impl_2__extend_from_slice #u8
+      #Alloc.Alloc.t_Global
+      out
+      (self.f_metadata_sk <: t_Slice u8)
+  in
+  let out:Alloc.Vec.t_Vec u8 Alloc.Alloc.t_Global =
+    Alloc.Vec.impl_2__extend_from_slice #u8
+      #Alloc.Alloc.t_Global
+      out
+      (self.f_metadata_pk <: t_Slice u8)
+  in
+  out
+
+/// Deserialize from
+/// `apke_dhakem_sk || apke_mlkem_sk || apke_mlkem_pk || metadata_sk || metadata_pk` bytes.
+/// # Errors
+/// Returns an error if the byte slice has the incorrect length.
+let impl_EphemeralBundleBytes__from_bytes (bytes: t_Slice u8)
+    : Core_models.Result.t_Result t_EphemeralBundleBytes Anyhow.t_Error =
+  if (Core_models.Slice.impl__len #u8 bytes <: usize) <>. impl_EphemeralBundleBytes__LEN
+  then
+    let args:(usize & usize) =
+      impl_EphemeralBundleBytes__LEN, Core_models.Slice.impl__len #u8 bytes <: (usize & usize)
+    in
+    let args:t_Array Core_models.Fmt.Rt.t_Argument (mk_usize 2) =
+      let list =
+        [
+          Core_models.Fmt.Rt.impl__new_display #usize args._1;
+          Core_models.Fmt.Rt.impl__new_display #usize args._2
+        ]
+      in
+      FStar.Pervasives.assert_norm (Prims.eq2 (List.Tot.length list) 2);
+      Rust_primitives.Hax.array_of_list 2 list
+    in
+    Core_models.Result.Result_Err
+    (Anyhow.Error.impl__msg #Alloc.String.t_String
+        (Core_models.Hint.must_use #Alloc.String.t_String
+            (Alloc.Fmt.format (Core_models.Fmt.Rt.impl_1__new_v1 (mk_usize 2)
+                    (mk_usize 2)
+                    (let list = ["Invalid EphemeralBundleBytes length: expected "; ", got "] in
+                      FStar.Pervasives.assert_norm (Prims.eq2 (List.Tot.length list) 2);
+                      Rust_primitives.Hax.array_of_list 2 list)
+                    args
+                  <:
+                  Core_models.Fmt.t_Arguments)
+              <:
+              Alloc.String.t_String)
+          <:
+          Alloc.String.t_String))
+    <:
+    Core_models.Result.t_Result t_EphemeralBundleBytes Anyhow.t_Error
+  else
+    let (apke_dhakem_sk: t_Slice u8), (rest: t_Slice u8) =
+      Core_models.Slice.impl__split_at #u8 bytes (mk_usize 32)
+    in
+    let (apke_mlkem_sk: t_Slice u8), (rest: t_Slice u8) =
+      Core_models.Slice.impl__split_at #u8
+        rest
+        Securedrop_protocol_minimal.Primitives.Mlkem.v_MLKEM768_PRIVATE_KEY_LEN
+    in
+    let (apke_mlkem_pk: t_Slice u8), (rest: t_Slice u8) =
+      Core_models.Slice.impl__split_at #u8
+        rest
+        Securedrop_protocol_minimal.Primitives.Mlkem.v_MLKEM768_PUBLIC_KEY_LEN
+    in
+    let (metadata_sk: t_Slice u8), (metadata_pk: t_Slice u8) =
+      Core_models.Slice.impl__split_at #u8
+        rest
+        Securedrop_protocol_minimal.Primitives.Xwing.v_XWING_PRIVATE_KEY_LEN
+    in
+    Core_models.Result.Result_Ok
+    ({
+        f_apke_dhakem_sk
+        =
+        Core_models.Result.impl__expect #(t_Array u8 (mk_usize 32))
+          #Core_models.Array.t_TryFromSliceError
+          (Core_models.Convert.f_try_into #(t_Slice u8)
+              #(t_Array u8 (mk_usize 32))
+              #FStar.Tactics.Typeclasses.solve
+              apke_dhakem_sk
+            <:
+            Core_models.Result.t_Result (t_Array u8 (mk_usize 32))
+              Core_models.Array.t_TryFromSliceError)
+          "wrong checked length";
+        f_apke_mlkem_sk
+        =
+        Core_models.Result.impl__expect #(t_Array u8 (mk_usize 2400))
+          #Core_models.Array.t_TryFromSliceError
+          (Core_models.Convert.f_try_into #(t_Slice u8)
+              #(t_Array u8 (mk_usize 2400))
+              #FStar.Tactics.Typeclasses.solve
+              apke_mlkem_sk
+            <:
+            Core_models.Result.t_Result (t_Array u8 (mk_usize 2400))
+              Core_models.Array.t_TryFromSliceError)
+          "wrong checked length";
+        f_apke_mlkem_pk
+        =
+        Core_models.Result.impl__expect #(t_Array u8 (mk_usize 1184))
+          #Core_models.Array.t_TryFromSliceError
+          (Core_models.Convert.f_try_into #(t_Slice u8)
+              #(t_Array u8 (mk_usize 1184))
+              #FStar.Tactics.Typeclasses.solve
+              apke_mlkem_pk
+            <:
+            Core_models.Result.t_Result (t_Array u8 (mk_usize 1184))
+              Core_models.Array.t_TryFromSliceError)
+          "wrong checked length";
+        f_metadata_sk
+        =
+        Core_models.Result.impl__expect #(t_Array u8 (mk_usize 32))
+          #Core_models.Array.t_TryFromSliceError
+          (Core_models.Convert.f_try_into #(t_Slice u8)
+              #(t_Array u8 (mk_usize 32))
+              #FStar.Tactics.Typeclasses.solve
+              metadata_sk
+            <:
+            Core_models.Result.t_Result (t_Array u8 (mk_usize 32))
+              Core_models.Array.t_TryFromSliceError)
+          "wrong checked length";
+        f_metadata_pk
+        =
+        Core_models.Result.impl__expect #(t_Array u8 (mk_usize 1216))
+          #Core_models.Array.t_TryFromSliceError
+          (Core_models.Convert.f_try_into #(t_Slice u8)
+              #(t_Array u8 (mk_usize 1216))
+              #FStar.Tactics.Typeclasses.solve
+              metadata_pk
+            <:
+            Core_models.Result.t_Result (t_Array u8 (mk_usize 1216))
+              Core_models.Array.t_TryFromSliceError)
+          "wrong checked length"
+      }
+      <:
+      t_EphemeralBundleBytes)
+    <:
+    Core_models.Result.t_Result t_EphemeralBundleBytes Anyhow.t_Error
